\documentclass{article}
\usepackage{pdflscape}
\usepackage[table]{xcolor}
\usepackage{amsmath, amssymb, amsthm}
\newcommand{\Mod}[1]{\ (\text{mod}\ #1)}
\newcommand{\R}{\mathbb{R}}
\newcommand{\N}{\mathbb{N}}
\newcommand{\Q}{\mathbb{Q}}
\newcommand{\E}{\mathbb{E}}
\newcommand{\F}{\mathbb{F}}
\newcommand{\Z}{\mathbb{Z}}
\newcommand{\mC}{\mathcal{C}}
\newcommand{\borel}{\mathcal{B}(\R)}
\newcommand{\mS}{\mathcal{S}}
\renewcommand{\P}{\mathbb{P}}
\DeclareMathOperator{\Span}{Span}
\DeclareMathOperator{\geom}{Geom}
\DeclareMathOperator{\vari}{Var}
	
\definecolor{lightgray}{gray}{0.95}
\begin{document}
\begin{landscape}
\centering % Center table
\begin{table}[]
\centering
\rowcolors{1}{}{lightgray}
\begin{tabular}{lr r r r r r r}
\hline
Distributions &  PMF/PDF&  CDF& MGF&  $\E[X]$&  $\vari(X)$&  $\E[X^2]$\\
\hline
\vspace{0.3cm}
$B(p)$& $f(x) = \begin{cases} 1-p &x=0\\p &x=1\end{cases}$ & $F(x) = \begin{cases}0 & x<0 \\ 1-p &0\leq x < 1\\1 & x \geq 1\end{cases}$ & $M(s) = (1-p) + pe^s$ &  $p$&  $p(1-p)$& $p$ \\
\vspace{0.3cm}
$B(n,p)$&  $f(k) = \binom{n}{k}p^k(1-p)^{n-k}$&  $F(k) = \sum_{i=0}^{\lfloor k \rfloor}\binom{n}{i} p^i(1-p)^{n-i}$& $M(s) = (pe^s +1 -p)^n$ &  $np$& $np(1-p)$ & $np(p(n-1)+1)$ \\
\vspace{0.3cm}
$P(\lambda)$&  $f(k) = e^{-\lambda}\frac{\lambda^k}{k!}$&  $F(k) = \sum_{i=0}^{\lfloor k \rfloor}e^{-\lambda}\frac{\lambda^i}{i!}$& $M(s) = e^{(e^s-1)\lambda}$&  $\lambda$&  $\lambda$& $\lambda^2+\lambda$ \\
\vspace{0.3cm}
$\geom(p)$&  $f(k) = (1-p)^kp$& $1-(1-p)^{k+1}$& $M(s) = \frac{p}{1-(e^s(1-p))}$ & $\frac{1-p}{p}$ & $\frac{1-p}{p^2}$ &$\frac{(p-1)(p-2)}{p^2}$ \\
\vspace{0.3cm}
$U(a.b)$&  $f(x) = \mathbb{1}_{(a,b)}(x)\cdot\frac{1}{b-a}$&  $F(x) = \begin{cases} 0 & x\leq a\\ \frac{x-a}{b-a} & a < x<b \\ 1 & x \geq b \end{cases}$&  $M(s) = \frac{e^{sb}-e^{sa}}{s(b-a)}$&  $\frac{a+b}{2}$&  $\frac{(b-a)^2}{12}$&$\frac{(b-a)^2+3(a+b)^2}{12}$\\
\vspace{0.3cm}
$\exp(\lambda)$&  $f(x) = \lambda e^{\lambda x}$&  $F(x) = 1-e^{-\lambda x}$&$M(s) = \frac{\lambda}{\lambda -s}$ & $\frac{1}{\lambda}$&  $\frac{1}{\lambda^2}$ &$\frac{2}{\lambda^2}$  \\
\vspace{0.3cm}
$N(m,\sigma^2)$&  $f(x) = \frac{1}{\sqrt{2\pi \sigma^2}}e^{-\frac{(x-m)^2}{2\sigma^2}}$&  $F(x) = \int_{-\infty}^{x}\frac{1}{\sqrt{2\pi \sigma^2}}e^{-\frac{(x-m)^2}{2\sigma^2}}$&  $M(s) = \exp\left(ms+ \frac{\sigma^2 s^2}{2}\right)$&  $m$&  $\sigma^2$& $\sigma^2+m^2$ 
 
\end{tabular}
\end{table}
\end{landscape}
\end{document}